\documentclass{article}
\usepackage{amsmath} 
\usepackage{amssymb}
\begin{document} 
    \begin{titlepage}
    \begin{center}
    \line(1,0){300}\\
    [0.25 in]
    \huge{\bfseries Shihab Muhtasim}\\
    [0.5 cm]
    \textsc{\Large Student ID: 21301610}\\
    \line(1,0){400}\\
    [2 cm]
    \textsc{\LARGE MAT 110}\\
    [0.5 cm]
    \textsc{\LARGE ASSIGNMENT 04}\\
    [0.5 cm]
    \textsc{\LARGE SET 7}\\
    \end{center}
    \end{titlepage}
\begin{newpage}
    \begin{flushright}
    \textsc{Assignment 4}\\
    \textsc{Problem 1}\\
    [1 cm]
    \end{flushright}
\begin{center}
  \textbf{\Large \underline {Ans to the question no 01}}\\
  [0.5 cm]
\end{center}
\Large {Given function, \\[3mm]
$ f(x,y)=y\cdot e^{(xy+3x+2y^2)}$\\[3mm] 
Now,\\[3mm]  
$f_x=y\cdot e^{(xy+3x+2y^2)}\cdot(y+3)=(y^2+3y)\cdot e^{(xy+3x+2y^2)}\\[3mm]
f_y=e^{(xy+3x+2y^2)}+y\cdot e^{(xy+3x+2y^2)}\cdot (x+4y)\\[3mm]
\Rightarrow f_y= e^{(xy+3x+2y^2)}(1+xy+4y^2)\\[3mm]
f_{xx}=e^{(xy+3x+2y^2)} \cdot (y+3)\cdot y(y+3)=e^{(xy+3x+2y^2)} \cdot y(y+3)^2\\[3mm]
f_{yy}=e^{(xy+3x+2y^2)}\cdot (x+4y)\cdot (1+xy+4y^2)+e^{(xy+3x+2y^2)}\cdot (x+8y)\\[3mm]
\Rightarrow f_{yy}=e^{(xy+3x+2y^2)}\cdot \{(x+4y)(1+xy+4y^2)+(x+8y)\}\\[3mm]
f_{xy}=(2y+3)\cdot e^{(xy+3x+2y^2)} +(y^2+3y)\cdot e^{(xy+3x+2y^2)}\cdot (x+4y)\\[3mm]
\Rightarrow f_{xy}= e^{(xy+3x+2y^2)}\{(2y+3)+(y^2+3y)(x+4y)\}\\[3mm]$
Now,
$f(0,0)=0\\[3mm]
f_x(0,0)=0\\[3mm]
f_y(0,0)=1\\[3mm]
f_{xx}(0,0)=0\\[3mm]
f_{yy}(0,0)=0\\[3mm]
f_{xy}(0,0)=3$\\[10mm]
The first degree Maclaurin polynomial approximation,\\[3mm]
$\therefore L(x,y)=f(0,0)+f_x(0,0)(x-0)+f_y(0,0)(y-0)\\[3mm]
\Rightarrow L(x,y)=0+0+1\cdot y=y\\[3mm]
\therefore  L(x,y)=y$\\[3mm]
The second degree Maclaurin polynomial approximation,\\[3mm]
$Q(x,y)=L(x,y)+\frac{f_{xx}(0,0)}{2!}\cdot (x-0)^2+\frac{f_{yy}(0,0)}{2!}\cdot(y-0)^2+\frac{f_{xy}(0,0)}{1!}\cdot(x-0)(y-0)\\[3mm]
\Rightarrow Q(x,y)=y+0+0+3xy=y(3x+1)\\[3mm]
\therefore Q(x,y)=y(3x+1)\\[3mm]$} 
\end{newpage}
\begin{newpage}
    \begin{flushright}
    \textsc{Assignment 4}\\
    \textsc{Problem 2}\\
    [1 cm]
    \end{flushright}
\begin{center}
  \textbf{\Large \underline {Ans to the question no 02}}\\
  [0.5 cm]
\end{center}
\Large {Given function, \\[3mm]
$ f(x,y)=f(x,y) = 4xye^{-x^2-y^2}$\\[3mm]
Now,\\[2mm]
$f_x=4y \cdot \{e^{-x^2-y^2}+xe^{-x^2-y^2}(-2x)\}\\[3mm]
\Rightarrow f_x=4y\cdot e^{-x^2-y^2}(1-2x^2)\\[3mm]
f_y=4x \cdot \{e^{-x^2-y^2}+ye^{-x^2-y^2}(-2x)\}\\[3mm]
\Rightarrow f_y=4x\cdot e^{-x^2-y^2}(1-2y^2)\\[3mm]$
For extreme values,\\[3mm]
$f_x=0\\[3mm]
\Rightarrow 4y\cdot e^{-x^2-y^2}(1-2x^2) =0 \\[3mm]
e^{-x^2-y^2}$ cannot be zero for any finite values of x or y\\[3mm]
$\therefore y=0$ or $x=\pm \frac{1}{\sqrt{2}}$\\[3mm]
Similarly,\\[3mm]
$f_y=0\\[3mm]
\Rightarrow 4x\cdot e^{-x^2-y^2}(1-2y^2) =0 \\[3mm]
e^{-x^2-y^2}$ cannot be zero for any finite values of x or y\\[3mm]
$\therefore x=0$ or $y=\pm \frac{1}{\sqrt{2}}$\\[3mm]
The critical points are: $(0,0),(0,\frac{1}{\sqrt{2}}),(0,-\frac{1}{\sqrt{2}}),(\frac{1}{\sqrt{2}},0)\\[3mm]
(-\frac{1}{\sqrt{2}},0),(\frac{1}{\sqrt{2}},\frac{1}{\sqrt{2}}),(\frac{1}{\sqrt{2}},-\frac{1}{\sqrt{2}}),(-\frac{1}{\sqrt{2}},+\frac{1}{\sqrt{2}}),(-\frac{1}{\sqrt{2}},-\frac{1}{\sqrt{2}})$\\[3mm]
Now,\\[3mm]
$f_{xx}=4y\{e^{-x^2-y^2}(-4x)+(1-2x^2)e^{-x^2-y^2}(-2x)\} \\[3mm]
\Rightarrow f_{xx}=4y\{2xe^{-x^2-y^2}(2x^2-3)\}\\[3mm]
\Rightarrow f_{xx}=8xy(2x^2-3)e^{-x^2-y^2}\\[3mm]
f_{yy}=4x\{e^{-x^2-y^2}(-4y)+(1-2y^2)e^{-x^2-y^2}(-2y)\} \\[3mm]
\Rightarrow f_{xx}=4x\{2xe^{-x^2-y^2}(2y^2-3)\}\\[3mm]
\Rightarrow f_{xx}=8xy(2y^2-3)e^{-x^2-y^2}\\[3mm]
f_{xy}=4\{e^{-x^2-y^2}(1-2x^2)+ye^{-x^2-y^2}(-2y)(1-2x^2)\}\\[3mm]
\Rightarrow f_{xy}=4e^{-x^2-y^2}(1-2x^2)(1-2y^2)$\\[3mm]
For $(0,0),\\[3mm]
A=f_{xx}(0,0)=0\\[3mm]
B=f_{xy}(0,0)=4\\[3mm]
C=f_{yy}(0,0)=0\\[3mm]
D=AC-B^2=0-4^2=-16\\[3mm]$
Since $D<0$, f has a saddle point at (0,0)\\[3mm]
For $(0,\frac{1}{\sqrt{2}}),\\[3mm]
A=f_{xx}(0,\frac{1}{\sqrt{2}})=0\\[3mm]
B=f_{xy}(0,\frac{1}{\sqrt{2}})=0\\[3mm]
C=f_{yy}(0,\frac{1}{\sqrt{2}})=0\\[3mm]
D=AC-B^2=0\\[3mm]$
Since $D=0$, No conclusion can be done\\[3mm]
For $(0,-\frac{1}{\sqrt{2}}),\\[3mm]
A=f_{xx}(0,-\frac{1}{\sqrt{2}})=0\\[3mm]
B=f_{xy}(0,-\frac{1}{\sqrt{2}})=0\\[3mm]
C=f_{yy}(0,-\frac{1}{\sqrt{2}})=0\\[3mm]
D=AC-B^2=0\\[3mm]$
Since $D=0$, No conclusion can be done\\[3mm]
For $(\frac{1}{\sqrt{2}},0),\\[3mm]
A=f_{xx}(\frac{1}{\sqrt{2}},0)=0\\[3mm]
B=f_{xy}(\frac{1}{\sqrt{2}},0)=0\\[3mm]
C=f_{yy}(\frac{1}{\sqrt{2}},0)=0\\[3mm]
D=AC-B^2=0\\[3mm]$
Since $D=0$, No conclusion can be done\\[3mm]
For $(-\frac{1}{\sqrt{2}},0),\\[3mm]
A=f_{xx}(-\frac{1}{\sqrt{2}},0)=0\\[3mm]
B=f_{xy}(-\frac{1}{\sqrt{2}},0)=0\\[3mm]
C=f_{yy}(-\frac{1}{\sqrt{2}},0)=0\\[3mm]
D=AC-B^2=0\\[3mm]$
Since $D=0$, No conclusion can be done\\[3mm]
For $(\frac{1}{\sqrt{2}},\frac{1}{\sqrt{2}}),\\[3mm]
A=f_{xx}(\frac{1}{\sqrt{2}},\frac{1}{\sqrt{2}})=-8e^{-1}=-2.943\\[3mm]
B=f_{xy}(\frac{1}{\sqrt{2}},\frac{1}{\sqrt{2}})=0\\[3mm]
C=f_{yy}(\frac{1}{\sqrt{2}},\frac{1}{\sqrt{2}})=-8e^{-1}=-2.943\\[3mm]
D=AC-B^2=8.66\\[3mm]$
Since $D>0$ and $A<0$, f has a relative maximum point at $(\frac{1}{\sqrt{2}},\frac{1}{\sqrt{2}})$\\[3mm]
For $(\frac{1}{\sqrt{2}},-\frac{1}{\sqrt{2}}),\\[3mm]
A=f_{xx}(\frac{1}{\sqrt{2}},-\frac{1}{\sqrt{2}})=8e^{-1}=2.943\\[3mm]
B=f_{xy}(\frac{1}{\sqrt{2}},-\frac{1}{\sqrt{2}})=0\\[3mm]
C=f_{yy}(\frac{1}{\sqrt{2}},-\frac{1}{\sqrt{2}})=8e^{-1}=2.943\\[3mm]
D=AC-B^2=8.66\\[3mm]$
Since $D>0$ and $A>0$, f has a relative minimum point at $(\frac{1}{\sqrt{2}},-\frac{1}{\sqrt{2}})$\\[3mm]
For $(-\frac{1}{\sqrt{2}},\frac{1}{\sqrt{2}}),\\[3mm]
A=f_{xx}(-\frac{1}{\sqrt{2}},\frac{1}{\sqrt{2}})=8e^{-1}=2.943\\[3mm]
B=f_{xy}(-\frac{1}{\sqrt{2}},\frac{1}{\sqrt{2}})=0\\[3mm]
C=f_{yy}(-\frac{1}{\sqrt{2}},\frac{1}{\sqrt{2}})=8e^{-1}=2.943\\[3mm]
D=AC-B^2=8.66\\[3mm]$
Since $D>0$ and $A>0$, f has a relative minimum point at $(-\frac{1}{\sqrt{2}},\frac{1}{\sqrt{2}})$\\[3mm]
For $(-\frac{1}{\sqrt{2}},-\frac{1}{\sqrt{2}}),\\[3mm]
A=f_{xx}(-\frac{1}{\sqrt{2}},-\frac{1}{\sqrt{2}})=-8e^{-1}=-2.943\\[3mm]
B=f_{xy}(-\frac{1}{\sqrt{2}},-\frac{1}{\sqrt{2}})=0\\[3mm]
C=f_{yy}(-\frac{1}{-\sqrt{2}},-\frac{1}{\sqrt{2}})=-8e^{-1}=-2.943\\[3mm]
D=AC-B^2=8.66\\[3mm]$
Since $D>0$ and $A<0$, f has a relative maximum point at $(-\frac{1}{\sqrt{2}},-\frac{1}{\sqrt{2}})$\\[3mm]
$\therefore$ Saddle point:(0,0)\\[3mm]
Maxima:$(-\frac{1}{\sqrt{2}},-\frac{1}{\sqrt{2}})$,$(\frac{1}{\sqrt{2}},\frac{1}{\sqrt{2}})$\\[3mm]
Minima:$(\frac{1}{\sqrt{2}},-\frac{1}{\sqrt{2}})$,$(-\frac{1}{\sqrt{2}},\frac{1}{\sqrt{2}})$ \\[3mm]}
\end{newpage}
\begin{newpage}
    \begin{flushright}
    \textsc{Assignment 4}\\
    \textsc{Problem 3}\\
    [1 cm]
    \end{flushright}
\begin{center}
  \textbf{\Large \underline {Ans to the question no 03}}\\
  [0.5 cm]
\end{center}
\Large {Given function, \\[3mm]
$ x-2y + z = 16
\Rightarrow z=16-x+2y$\\[3mm]
At origin (0,0),\\[3mm]
$D=(Distance)^2=(x-0)^2+(y-0)^2+(z-0)^2\\[3mm]
=x^2+y^2+z^2\\[3mm]
=x^2+y^2+(16-x+2y)^2$\\[3mm]
Here,\\[3mm]
$D_x=2x+2(16-x+2y)(-1)\\[3mm]
=2x-32+2x-4y\\[3mm]
=4x-4y-32\\[3mm]$
When $D_x=0,\\[3mm]
4x-4y-32=0\\[3mm]
\Rightarrow x-y-8=0\\[3mm]
\Rightarrow y=x-8\\[3mm]$
Again,
$D_y=2y+2(16-x+2y)(2)\\[3mm]
=2y+64-4x+8y\\[3mm]
=10y-4x+64\\[3mm]$
When $D_y=0\\[3mm]
10y-4x+64=0\\[3mm]
\Rightarrow 5(x-8)-4x+64=0\\[3mm]
\Rightarrow 3x-8=0 \\[3mm]
\Rightarrow x=\frac{8}{3}\\[3mm]$
Substituting the value of x in the equation $ y=x-8,\\[3mm]
y=\frac{-16}{3}\\[3mm]
\therefore (x,y)=(\frac{8}{3},\frac{-16}{3})\\[3mm]$
Now,
$A=D_{xx}=4\\[3mm]
C=D_{yy}=10\\[3mm]
B=D_{xy}=-4\\[3mm]
D=AC-B^2=24\\[3mm]$
Since $D>0$ and $A>0$, D has a minimum at point $(\frac{8}{3},\frac{-16}{3})$\\[3mm]
Now, \\[3mm]
$D(\frac{8}{3},\frac{-16}{3})=(\frac{8}{3})^2+(\frac{-16}{3})^2+(16-\frac{8}{3}-\frac{2\cdot 16}{3})^2\\[3mm]
=\frac{64}{9}+\frac{256}{9}+(\frac{40}{3}-\frac{32}{3})^2\\[3mm]
=\frac{64}{9}+\frac{256}{9}+(\frac{8}{3})^2\\[3mm]
=\frac{128}{9}+\frac{256}{9}\\[3mm]
=\frac{128}{3}\\[3mm]
\therefore Distance= \sqrt{\frac{128}{3}}=\frac{8\sqrt{6}}{3}\\[3mm]
Since, x=\frac{8}{3}, y=\frac{-16}{3},\\[3mm]
z=16-\frac{8}{3}+\frac{2\cdot-16}{3}=\frac{8}{3}\\[3mm]$
the point in the given plane that is closest to the origin is$(\frac{8}{3},\frac{-16}{3},\frac{8}{3})\\[3mm]$}
\end{newpage}
\begin{newpage}
    \begin{flushright}
    \textsc{Assignment 4}\\
    \textsc{Problem 4}\\
    [1 cm]
    \end{flushright}
\begin{center}
  \textbf{\Large \underline {Ans to the question no 04}}\\
  [0.5 cm]
\end{center}
\Large {Given function, \\[3mm]
$ \vec{F}=-x^{2}(y-z) \hat{i}-\left(x^{2}+y^{4}\right) \hat{j}+\left(\frac{4 z^{2}}{y^{2}}\right)\hat{k}\\[3mm]
\Rightarrow \vec{F}=(-x^{2}y+-x^{2}z) \hat{i}+\left(-x^{2}-y^{4}\right) \hat{j}+\left(4 z^{2}y^{-2}\right)\hat{k}\\[3mm]$
Curl $\vec{F}=\left|\begin{array}{ccc}\hat{i} & \hat{j} & \hat{k}\\
\frac{\partial}{\partial x} & \frac{\partial}{\partial y} & \frac{\partial}{\partial z} \\
-x^{2}y+x^{2}z & -x^{2}-y^{4} & 4 z^{2} y^{-2}
\end{array}\right|\\[3mm]
=\hat{i}\{\frac{\partial}{\partial y}(4 z^{2} y^{-2})-\frac{\partial}{\partial z}(-x^{2}-y^{4})\}-\hat{j}\{\frac{\partial}{\partial x}(4 z^{2} y^{-2})-{\frac{\partial}{\partial z}}(-x^{2}y+x^{2}z)+\hat{k}\{\frac{\partial}{\partial x}(-x^{2}-y^{4})-\frac{\partial}{\partial y}(-x^{2}y+x^{2}z)\}\\[3mm]
=(-8z^2y^{-3})\hat{i}-(0-0+x^2)\hat{j}+(-2x+x^2)\hat{k}\\[3mm]
=-8z^2y^{-3}\hat{i}-x^2\hat{j}-(2x+x^2)\hat{k}$\\[3mm]
Div $\vec{F}=\Delta F\\[3mm]
=\frac{\partial F_x}{\partial x}+\frac{\partial F_y}{\partial y}+\frac{\partial F_z}{\partial z}\\[3mm]
=\frac{\partial }{\partial x}(-x^{2}y+-x^{2}z)+\frac{\partial}{\partial y}(-x^{2}-y^{4})+\frac{\partial}{\partial z}(4 z^{2}y^{-2})\\[3mm]
=-2x(y-z)-4y^3+\frac{8z}{y^2}\\[3mm]
\therefore Curl \vec{F}=-8z^2y^{-3}\hat{i}-x^2\hat{j}-(2x+x^2)\hat{k}\\[3mm]
\therefore \Delta F=-2x(y-z)-4y^3+\frac{8z}{y^2}$}
\end{newpage}
\begin{newpage}
    \begin{flushright}
    \textsc{Assignment 4}\\
    \textsc{Problem 5}\\
    [1 cm]
    \end{flushright}
\begin{center}
  \textbf{\Large \underline {Ans to the question no 05}}\\
  [0.5 cm]
\end{center}
\Large {Given function, \\[3mm]
$ \vec{F} = 2yz\hat{i}-x^2y\hat{j} + xz^2\hat{k}\\[3mm]
\phi =2x^2yz^3\\[3mm]
\nabla \phi = (\frac{\partial}{\partial x}\hat{i}+\frac{\partial }{\partial y}\hat{j}+\frac{\partial }{\partial z}\hat{k}) \cdot (2x^2yz^3)\\[3mm]
=\frac{\partial}{\partial x}(2x^2yz^3)\hat{i}+\frac{\partial}{\partial y}(2x^2yz^3)\hat{j}+\frac{\partial}{\partial z}(2x^2yz^3)\hat{k}\\[3mm]
=4xyz^3\hat{i}+2x^2z^3\hat{j}+6x^2yz^2\hat{j}$\\[3mm]
Now,\\[3mm]
$\vec{F}\cdot (\nabla \phi)=(2yz\hat{i}-x^2y\hat{j} + xz^2\hat{k}) \cdot (4xyz^3\hat{i}+2x^2z^3\hat{j}+6x^2yz^2\hat{j})\\[3mm]
=8xy^2z^4-2x^4yz^3+6x^3yz^4\\[5mm]
\therefore \vec{F}\cdot (\nabla \phi)=8xy^2z^4-2x^4yz^3+6x^3yz^4$}
\end{newpage}
\begin{newpage}
    \begin{flushright}
    \textsc{Assignment 4}\\
    \textsc{Problem 6}\\
    [1 cm]
    \end{flushright}
\begin{center}
  \textbf{\Large \underline {Ans to the question no 06}}\\
  [0.5 cm]
\end{center}
\Large {Given function, \\[3mm]
$f(x,y,x)=x^2y + y^2z + xz^2\\[3mm]
\nabla \cdot f(x,y,x)=(\frac{\partial f}{\partial x}\hat{i}+\frac{\partial f}{\partial y}\hat{j}+\frac{\partial f}{\partial z}\hat{k})\\[3mm]
=\frac{\partial}{\partial x}(x^2y + y^2z + xz^2)\hat{i}+\frac{\partial f}{\partial y}(x^2y + y^2z + xz^2)\hat{j}+\frac{\partial f}{\partial z}(x^2y + y^2z + xz^2)\hat{k})\\[2mm]
=(2xy+z^2)\hat{i}+(x^2+2yz)\hat{j}+(y^2+2zx)\hat{k}\\[3mm]$
At the point (2,4,5),\\[3mm]
$\nabla \cdot f(2,4,5)=(2\cdot 2\cdot 4+5^2)\hat{i}+(2^2+2\cdot 4\cdot 5)\hat{j}+(4^2+2\cdot 5\cdot 2)\hat{k}\\[3mm]
=41\hat{i}+44\hat{j}+36\hat{k}\\[3mm]$
unit vector along (1,-1,3),\\[3mm]
$\hat{u}=\frac{\hat{i}-\hat{j}+3\hat{k}}{\sqrt{1^2+1^2+3^2}}\\[3mm]
=\frac{\hat{i}-\hat{j}+3\hat{k}}{\sqrt{11}}\\[3mm]$
Directional derivative of the function f(x,y,z) at the point (2,4,5) in the direction of the point (1,-1,3),\\[3mm]
$ (\nabla \cdot f(2,4,5))\cdot \hat{u}= \frac{41-44+108}{\sqrt{11}}\\[3mm]
=\frac{105}{\sqrt{11}}=31.66$}
\end{newpage}
\end{document}